fully define CBOR C types with custom unions, etc.

src/cbor/CBOR.SteelC.fst
@@ -1,74 +1,381 @@
 module CBOR.SteelC
 
+module Cbor = CBOR.Spec
 module Cs = Steel.ST.C.Types.UserStruct
+module Cu = Steel.ST.C.Types.UserUnion
+module F = Steel.ST.C.Types.Fields
 module C = Steel.ST.C.Types
 module U64 = FStar.UInt64
 module U8 = FStar.UInt8
 module SZ = FStar.SizeT
+module RW = Steel.ST.C.Rewrite
 
-inline_for_extraction
 noextract
-type union_item ([@@@strictly_positive] t: Type) (p: option bool) (one: t) = (x: t {
-  match p with
-  | None -> True
-  | Some p -> not p == FStar.StrongExcludedMiddle.strong_excluded_middle (x == one)
-})
+inline_for_extraction
+[@@ F.norm_field_attr]
+let cbor_string_fields =
+  F.field_description_cons "byte_length" (C.scalar U64.t) (
+  F.field_description_cons "payload" (C.scalar (C.array (C.scalar U8.t)))
+  F.field_description_nil)
 
-[@@erasable]
-noeq
-type cbor_case_tag =
-| CBORCaseInt64
-| CBORCaseString
-| CBORCaseTagged
-| CBORCaseArray
-| CBORCaseMap
-| CBORCaseSimpleValue
-| CBORCaseSerialized
+let cbor_string = C.struct_t "" cbor_string_fields
 
-noeq
-type cbor_string = {
-  cbor_string_byte_length: C.scalar_t U64.t;
-  cbor_string_payload: C.scalar_t (C.array (C.scalar U8.t));
-}
+noextract
+let cbor_string_td : C.typedef cbor_string = C.struct0 _ _ _
 
-noeq
-type cbor_serialized = {
-  cbor_serialized_byte_size: C.scalar_t SZ.t;
-  cbor_serialized_payload: C.scalar_t (C.array (C.scalar U8.t));
-}
+noextract
+inline_for_extraction
+[@@ F.norm_field_attr]
+let cbor_serialized_fields =
+  F.field_description_cons "byte_size" (C.scalar SZ.t) (
+  F.field_description_cons "payload" (C.scalar (C.array (C.scalar U8.t)))
+  F.field_description_nil)
 
-let cbor_serialized_one : Ghost.erased cbor_serialized = Ghost.hide {
-  cbor_serialized_byte_size = C.unknown (C.scalar SZ.t);
-  cbor_serialized_payload = C.unknown (C.scalar (C.array (C.scalar U8.t)));
-}
+let cbor_serialized = C.struct_t "" cbor_serialized_fields
+
+noextract
+let cbor_serialized_td : C.typedef cbor_serialized = C.struct0 _ _ _
+
+noextract
+let cbor_case_known_tag : Cs.nonempty_set string =
+  FStar.Set.empty
+  `Cs.set_snoc` "cbor_case_int64"
+  `Cs.set_snoc` "cbor_case_string"
+  `Cs.set_snoc` "cbor_case_tagged"
+  `Cs.set_snoc` "cbor_case_array"
+  `Cs.set_snoc` "cbor_case_map"
+  `Cs.set_snoc` "cbor_case_simple_value"
+  `Cs.set_snoc` "cbor_case_serialized"
 
 noeq
 type cbor_tagged (active: Ghost.erased (option bool)) = {
-  cbor_tagged_tag: union_item (C.scalar_t U64.t) active (C.unknown (C.scalar U64.t));
-  cbor_tagged_payload: union_item (C.scalar_t (C.ptr_gen cbor)) active (C.unknown (C.scalar (C.ptr_gen cbor)));
+  cbor_tagged_tag: C.scalar_t U64.t;
+  cbor_tagged_payload: C.scalar_t (C.ptr_gen cbor);
+  cbor_tagged_active: squash (match Ghost.reveal active with
+  | None -> True
+  | Some tag_active -> (tag_active == false <==> (cbor_tagged_tag == C.unknown (C.scalar U64.t) /\ cbor_tagged_payload == C.unknown (C.scalar (C.ptr_gen cbor))))
+  );
 }
 and cbor_array (active: Ghost.erased (option bool)) = {
-  cbor_array_count: union_item (C.scalar_t U64.t) active (C.unknown (C.scalar U64.t));
-  cbor_array_payload: union_item (C.scalar_t (C.array_ptr_gen cbor)) active (C.unknown (C.scalar (C.array_ptr_gen cbor)));
+  cbor_array_count: C.scalar_t U64.t;
+  cbor_array_payload: C.scalar_t (C.array_ptr_gen cbor);
+  cbor_array_active: squash (match Ghost.reveal active with
+  | None -> True
+  | Some tag_active -> (tag_active == false <==> (cbor_array_count == C.unknown (C.scalar U64.t) /\ cbor_array_payload == C.unknown (C.scalar (C.array_ptr_gen cbor))))
+  );
 }
 and cbor_map (active: Ghost.erased (option bool)) = {
   cbor_map_entry_count: C.scalar_t U64.t;
   cbor_map_payload: C.scalar_t (C.ptr_gen cbor_pair);
+  cbor_map_active: squash (match Ghost.reveal active with
+  | None -> True
+  | Some tag_active -> (tag_active == false <==> (cbor_map_entry_count == C.unknown (C.scalar U64.t) /\ cbor_map_payload == C.unknown (C.scalar (C.ptr_gen cbor_pair))))
+  );
 }
 and cbor_case = { // TODO: find a way to extract this struct as an union
-  cbor_case_tag: cbor_case_tag;
-  cbor_case_int64: union_item (C.scalar_t U64.t) (Some (CBORCaseInt64? cbor_case_tag)) (C.unknown (C.scalar U64.t));
-  cbor_case_tagged: cbor_tagged (Some (CBORCaseTagged? cbor_case_tag));
-  cbor_case_array: cbor_array (Some (CBORCaseArray? cbor_case_tag));
-  cbor_case_map: cbor_map (Some (CBORCaseMap? cbor_case_tag));
-  cbor_case_simple_value: union_item (C.scalar_t U8.t) (Some (CBORCaseSimpleValue? cbor_case_tag)) (C.unknown (C.scalar U8.t));
-  cbor_case_serialized: union_item cbor_serialized (Some (CBORCaseSerialized? cbor_case_tag)) cbor_serialized_one;
+  cbor_case_tag: Ghost.erased (Cu.union_tag (Cs.set_def cbor_case_known_tag));
+  cbor_case_int64: Cu.union_item_t (C.scalar_t U64.t) (C.unknown (C.scalar U64.t)) (Some (Cu.TagKnown (Some "cbor_case_int64") = Ghost.reveal cbor_case_tag));
+  cbor_case_string: Cu.union_item_t cbor_string (C.unknown cbor_string_td) (Some (Cu.TagKnown (Some "cbor_case_string") = Ghost.reveal cbor_case_tag));
+  cbor_case_tagged: cbor_tagged (Some (Cu.TagKnown (Some "cbor_case_tagged") = Ghost.reveal cbor_case_tag));
+  cbor_case_array: cbor_array (Some (Cu.TagKnown (Some "cbor_case_array") = Ghost.reveal cbor_case_tag));
+  cbor_case_map: cbor_map (Some (Cu.TagKnown (Some "cbor_case_map") = Ghost.reveal cbor_case_tag));
+  cbor_case_simple_value: Cu.union_item_t (C.scalar_t Cbor.simple_value) (C.unknown (C.scalar Cbor.simple_value)) (Some (Cu.TagKnown (Some "cbor_case_simple_value") = Ghost.reveal cbor_case_tag));
+  cbor_case_serialized: Cu.union_item_t cbor_serialized (C.unknown cbor_serialized_td) (Some (Cu.TagKnown (Some "cbor_case_serialized") = Ghost.reveal cbor_case_tag));
+  cbor_case_unknown: Cu.union_item_t (C.scalar_t (squash False)) (C.unknown (C.scalar (squash False))) (Some (Cu.TagKnown None = Ghost.reveal cbor_case_tag));
 }
 and cbor = {
-  cbor_type: U8.t;
+  cbor_type: C.scalar_t Cbor.major_type_t;
   cbor_payload: cbor_case;
 }
 and cbor_pair = {
   cbor_pair_fst: cbor;
   cbor_pair_snd: cbor;
 }
+
+noextract
+inline_for_extraction
+[@@F.norm_field_attr]
+let cbor_tagged_struct_def : Cs.struct_def (cbor_tagged None) =
+  let fields = FStar.Set.empty `Cs.set_snoc` "cbor_tagged_tag" `Cs.set_snoc` "cbor_tagged_payload" in
+  let field_desc : Steel.ST.C.Types.Struct.Aux.field_description_gen_t (Cs.field_t fields) = {
+    fd_nonempty = Cs.nonempty_set_nonempty_type "cbor_tagged_tag" fields;
+    fd_type = (fun (n: Cs.field_t fields) -> match n with "cbor_tagged_tag" -> C.scalar_t U64.t | "cbor_tagged_payload" -> C.scalar_t (C.ptr_gen cbor));
+    fd_typedef = (fun (n: Cs.field_t fields) -> match n with "cbor_tagged_tag" -> C.scalar U64.t | "cbor_tagged_payload" -> C.scalar (C.ptr_gen cbor));
+  }
+  in {
+  fields = fields;
+  field_desc = field_desc;
+  mk = (fun f -> Mkcbor_tagged (f "cbor_tagged_tag") (f "cbor_tagged_payload") ());
+  get = (fun (x: cbor_tagged None) (f: Cs.field_t fields) -> match f with "cbor_tagged_tag" -> x.cbor_tagged_tag | "cbor_tagged_payload" -> x.cbor_tagged_payload);
+  get_mk = (fun _ _ -> ());
+  extensionality = (fun s1 s2 phi -> phi "cbor_tagged_tag"; phi "cbor_tagged_payload")
+}
+
+noextract
+let cbor_tagged_td : C.typedef (cbor_tagged None) = Cs.struct_typedef cbor_tagged_struct_def
+
+let cbor_tagged_unknown : Ghost.erased (cbor_tagged None) = Ghost.hide ({
+  cbor_tagged_tag = C.unknown (C.scalar U64.t);
+  cbor_tagged_payload = C.unknown (C.scalar (C.ptr_gen cbor));
+  cbor_tagged_active = ();
+})
+
+let cbor_tagged_unknown_eq : squash (C.unknown cbor_tagged_td == Ghost.reveal cbor_tagged_unknown) =
+  cbor_tagged_struct_def.extensionality (C.unknown (cbor_tagged_td)) (Ghost.reveal cbor_tagged_unknown) (fun _ -> ())
+
+noextract
+inline_for_extraction
+[@@F.norm_field_attr]
+let cbor_tagged_is_union_item : Cu.is_union_item cbor_tagged (C.unknown cbor_tagged_td) = {
+  some_to_none = (fun _ x -> Mkcbor_tagged x.cbor_tagged_tag x.cbor_tagged_payload ());
+  none_to_some = (fun x -> Mkcbor_tagged x.cbor_tagged_tag x.cbor_tagged_payload ());
+  none_to_some_inj = (fun x -> ());
+  some_to_none_inj = (fun _ x -> ());
+}
+
+noextract
+inline_for_extraction
+[@@F.norm_field_attr]
+let cbor_array_struct_def : Cs.struct_def (cbor_array None) =
+  let fields = FStar.Set.empty `Cs.set_snoc` "cbor_array_count" `Cs.set_snoc` "cbor_array_payload" in
+  let field_desc : Steel.ST.C.Types.Struct.Aux.field_description_gen_t (Cs.field_t fields) = {
+    fd_nonempty = Cs.nonempty_set_nonempty_type "cbor_array_count" fields;
+    fd_type = (fun (n: Cs.field_t fields) -> match n with "cbor_array_count" -> C.scalar_t U64.t | "cbor_array_payload" -> C.scalar_t (C.array_ptr_gen cbor));
+    fd_typedef = (fun (n: Cs.field_t fields) -> match n with "cbor_array_count" -> C.scalar U64.t | "cbor_array_payload" -> C.scalar (C.array_ptr_gen cbor));
+  }
+  in {
+  fields = fields;
+  field_desc = field_desc;
+  mk = (fun f -> Mkcbor_array (f "cbor_array_count") (f "cbor_array_payload") ());
+  get = (fun (x: cbor_array None) (f: Cs.field_t fields) -> match f with "cbor_array_count" -> x.cbor_array_count | "cbor_array_payload" -> x.cbor_array_payload);
+  get_mk = (fun _ _ -> ());
+  extensionality = (fun s1 s2 phi -> phi "cbor_array_count"; phi "cbor_array_payload")
+}
+
+noextract
+let cbor_array_td : C.typedef (cbor_array None) = Cs.struct_typedef cbor_array_struct_def
+
+let cbor_array_unknown : Ghost.erased (cbor_array None) = Ghost.hide ({
+  cbor_array_count = C.unknown (C.scalar U64.t);
+  cbor_array_payload = C.unknown (C.scalar (C.array_ptr_gen cbor));
+  cbor_array_active = ();
+})
+
+let cbor_array_unknown_eq : squash (C.unknown cbor_array_td == Ghost.reveal cbor_array_unknown) =
+  cbor_array_struct_def.extensionality (C.unknown (cbor_array_td)) (Ghost.reveal cbor_array_unknown) (fun _ -> ())
+
+noextract
+inline_for_extraction
+[@@F.norm_field_attr]
+let cbor_array_is_union_item : Cu.is_union_item cbor_array (C.unknown cbor_array_td) = {
+  some_to_none = (fun _ x -> Mkcbor_array x.cbor_array_count x.cbor_array_payload ());
+  none_to_some = (fun x -> Mkcbor_array x.cbor_array_count x.cbor_array_payload ());
+  none_to_some_inj = (fun x -> ());
+  some_to_none_inj = (fun _ x -> ());
+}
+
+noextract
+inline_for_extraction
+[@@F.norm_field_attr]
+let cbor_map_struct_def : Cs.struct_def (cbor_map None) =
+  let fields = FStar.Set.empty `Cs.set_snoc` "cbor_map_entry_count" `Cs.set_snoc` "cbor_map_payload" in
+  let field_desc : Steel.ST.C.Types.Struct.Aux.field_description_gen_t (Cs.field_t fields) = {
+    fd_nonempty = Cs.nonempty_set_nonempty_type "cbor_map_entry_count" fields;
+    fd_type = (fun (n: Cs.field_t fields) -> match n with "cbor_map_entry_count" -> C.scalar_t U64.t | "cbor_map_payload" -> C.scalar_t (C.ptr_gen cbor_pair));
+    fd_typedef = (fun (n: Cs.field_t fields) -> match n with "cbor_map_entry_count" -> C.scalar U64.t | "cbor_map_payload" -> C.scalar (C.ptr_gen cbor_pair));
+  }
+  in {
+  fields = fields;
+  field_desc = field_desc;
+  mk = (fun f -> Mkcbor_map (f "cbor_map_entry_count") (f "cbor_map_payload") ());
+  get = (fun (x: cbor_map None) (f: Cs.field_t fields) -> match f with "cbor_map_entry_count" -> x.cbor_map_entry_count | "cbor_map_payload" -> x.cbor_map_payload);
+  get_mk = (fun _ _ -> ());
+  extensionality = (fun s1 s2 phi -> phi "cbor_map_entry_count"; phi "cbor_map_payload")
+}
+
+noextract
+let cbor_map_td : C.typedef (cbor_map None) = Cs.struct_typedef cbor_map_struct_def
+
+let cbor_map_unknown : Ghost.erased (cbor_map None) = Ghost.hide ({
+  cbor_map_entry_count = C.unknown (C.scalar U64.t);
+  cbor_map_payload = C.unknown (C.scalar (C.ptr_gen cbor_pair));
+  cbor_map_active = ();
+})
+
+let cbor_map_unknown_eq : squash (C.unknown cbor_map_td == Ghost.reveal cbor_map_unknown) =
+  cbor_map_struct_def.extensionality (C.unknown (cbor_map_td)) (Ghost.reveal cbor_map_unknown) (fun _ -> ())
+
+noextract
+inline_for_extraction
+[@@F.norm_field_attr]
+let cbor_map_is_union_item : Cu.is_union_item cbor_map (C.unknown cbor_map_td) = {
+  some_to_none = (fun _ x -> Mkcbor_map x.cbor_map_entry_count x.cbor_map_payload ());
+  none_to_some = (fun x -> Mkcbor_map x.cbor_map_entry_count x.cbor_map_payload ());
+  none_to_some_inj = (fun x -> ());
+  some_to_none_inj = (fun _ x -> ());
+}
+
+noextract
+inline_for_extraction
+[@@F.norm_field_attr]
+let cbor_case_field_desc : F.field_description_t unit = {
+  fd_def = Cs.set_def cbor_case_known_tag;
+  fd_empty = false;
+  fd_type = (fun f -> match f with 
+  | "cbor_case_int64" -> C.scalar_t U64.t
+  | "cbor_case_string" -> cbor_string
+  | "cbor_case_tagged" -> cbor_tagged None
+  | "cbor_case_array" -> cbor_array None
+  | "cbor_case_map" -> cbor_map None
+  | "cbor_case_simple_value" -> C.scalar_t Cbor.simple_value 
+  | "cbor_case_serialized" -> cbor_serialized
+  | _ -> squash False
+  );
+  fd_typedef = (fun f -> match f with 
+  | "cbor_case_int64" -> C.scalar U64.t
+  | "cbor_case_string" -> cbor_string_td
+  | "cbor_case_tagged" -> cbor_tagged_td
+  | "cbor_case_array" -> cbor_array_td
+  | "cbor_case_map" -> cbor_map_td
+  | "cbor_case_simple_value" -> C.scalar Cbor.simple_value 
+  | "cbor_case_serialized" -> cbor_serialized_td
+  );
+}
+
+noextract
+inline_for_extraction
+[@@F.norm_field_attr]
+let cbor_case_union_field_desc : Cu.union_field_description_t cbor_case_field_desc = {
+  fd_union_type = (fun f -> match f with
+  | "cbor_case_int64" -> Cu.union_item_t (C.scalar_t U64.t) (C.unknown (C.scalar U64.t))
+  | "cbor_case_string" -> Cu.union_item_t cbor_string (C.unknown cbor_string_td)
+  | "cbor_case_tagged" -> cbor_tagged
+  | "cbor_case_array" -> cbor_array
+  | "cbor_case_map" -> cbor_map
+  | "cbor_case_simple_value" -> Cu.union_item_t (C.scalar_t Cbor.simple_value) (C.unknown (C.scalar Cbor.simple_value))
+  | "cbor_case_serialized" -> Cu.union_item_t cbor_serialized (C.unknown cbor_serialized_td)
+  );
+  fd_union_type_rewrite = (fun f -> match f with
+  | "cbor_case_int64" -> Cu.union_item_rewrite (C.unknown (C.scalar U64.t))
+  | "cbor_case_string" -> Cu.union_item_rewrite (C.unknown cbor_string_td)
+  | "cbor_case_tagged" -> RW.rewrite_id (cbor_tagged None)
+  | "cbor_case_array" -> RW.rewrite_id (cbor_array None)
+  | "cbor_case_map" -> RW.rewrite_id (cbor_map None)
+  | "cbor_case_simple_value" -> Cu.union_item_rewrite (C.unknown (C.scalar Cbor.simple_value))
+  | "cbor_case_serialized" -> Cu.union_item_rewrite (C.unknown cbor_serialized_td)
+  );
+  fd_union_item = (fun f -> match f with
+  | "cbor_case_int64" -> Cu.union_item_gen (C.scalar U64.t)
+  | "cbor_case_string" -> Cu.union_item_gen cbor_string_td
+  | "cbor_case_tagged" -> cbor_tagged_is_union_item
+  | "cbor_case_array" -> cbor_array_is_union_item
+  | "cbor_case_map" -> cbor_map_is_union_item
+  | "cbor_case_simple_value" -> Cu.union_item_gen (C.scalar Cbor.simple_value)
+  | "cbor_case_serialized" -> Cu.union_item_gen cbor_serialized_td
+  );
+}
+
+noextract
+inline_for_extraction
+[@@F.norm_field_attr]
+let cbor_case_union_def : Cu.union_def cbor_case unit = {
+  fields = cbor_case_field_desc;
+  field_desc = cbor_case_union_field_desc;
+  mk = (fun tag phi -> {
+    cbor_case_tag = tag;
+    cbor_case_int64 = phi (Some "cbor_case_int64");
+    cbor_case_string = phi (Some "cbor_case_string");
+    cbor_case_tagged = phi (Some "cbor_case_tagged");
+    cbor_case_array = phi (Some "cbor_case_array");
+    cbor_case_map = phi (Some "cbor_case_map");
+    cbor_case_simple_value = phi (Some "cbor_case_simple_value");
+    cbor_case_serialized = phi (Some "cbor_case_serialized");
+    cbor_case_unknown = phi None;
+  });
+  get_tag = (fun x -> x.cbor_case_tag);
+  get = (fun x tag' -> match tag' with
+  | Some "cbor_case_int64" -> x.cbor_case_int64
+  | Some "cbor_case_string" -> x.cbor_case_string
+  | Some "cbor_case_tagged" -> x.cbor_case_tagged
+  | Some "cbor_case_array" -> x.cbor_case_array
+  | Some "cbor_case_map" -> x.cbor_case_map
+  | Some "cbor_case_simple_value" -> x.cbor_case_simple_value
+  | Some "cbor_case_serialized" -> x.cbor_case_serialized
+  | None -> x.cbor_case_unknown
+  );
+  get_tag_mk = (fun tag phi -> ());
+  get_mk = (fun tag phi f -> ());
+  extensionality = (fun x1 x2 prf_tag phi ->
+    phi (Some "cbor_case_int64");
+    phi (Some "cbor_case_string");
+    phi (Some "cbor_case_tagged");
+    phi (Some "cbor_case_array");
+    phi (Some "cbor_case_map");
+    phi (Some "cbor_case_simple_value");
+    phi (Some "cbor_case_serialized");
+    phi None
+  );
+}
+
+noextract
+let cbor_case_td : C.typedef cbor_case = Cu.union_typedef cbor_case_union_def
+
+noextract
+inline_for_extraction
+[@@F.norm_field_attr]
+let cbor_struct_def : Cs.struct_def cbor =
+  let fields = FStar.Set.empty `Cs.set_snoc` "cbor_type" `Cs.set_snoc` "cbor_payload" in
+  let field_desc : Steel.ST.C.Types.Struct.Aux.field_description_gen_t (Cs.field_t fields) = {
+    fd_nonempty = Cs.nonempty_set_nonempty_type "cbor_type" fields;
+    fd_type = (fun (n: Cs.field_t fields) -> match n with "cbor_type" -> C.scalar_t Cbor.major_type_t | "cbor_payload" -> cbor_case);
+    fd_typedef = (fun (n: Cs.field_t fields) -> match n with "cbor_type" -> C.scalar Cbor.major_type_t | "cbor_payload" -> cbor_case_td);
+  }
+  in {
+  fields = fields;
+  field_desc = field_desc;
+  mk = (fun f -> Mkcbor (f "cbor_type") (f "cbor_payload"));
+  get = (fun (x: cbor) (f: Cs.field_t fields) -> match f with "cbor_type" -> x.cbor_type | "cbor_payload" -> x.cbor_payload);
+  get_mk = (fun _ _ -> ());
+  extensionality = (fun s1 s2 phi -> phi "cbor_type"; phi "cbor_payload")
+}
+
+noextract
+let cbor_td : C.typedef cbor = Cs.struct_typedef cbor_struct_def
+
+noextract
+inline_for_extraction
+[@@F.norm_field_attr]
+let cbor_pair_struct_def : Cs.struct_def cbor_pair =
+  let fields = FStar.Set.empty `Cs.set_snoc` "cbor_pair_fst" `Cs.set_snoc` "cbor_pair_snd" in
+  let field_desc : Steel.ST.C.Types.Struct.Aux.field_description_gen_t (Cs.field_t fields) = {
+    fd_nonempty = Cs.nonempty_set_nonempty_type "cbor_pair_fst" fields;
+    fd_type = (fun _ -> cbor);
+    fd_typedef = (fun _ -> cbor_td);
+  }
+  in {
+  fields = fields;
+  field_desc = field_desc;
+  mk = (fun f -> Mkcbor_pair (f "cbor_pair_fst") (f "cbor_pair_snd"));
+  get = (fun (x: cbor_pair) (f: Cs.field_t fields) -> match f with "cbor_pair_fst" -> x.cbor_pair_fst | "cbor_pair_snd" -> x.cbor_pair_snd);
+  get_mk = (fun _ _ -> ());
+  extensionality = (fun s1 s2 phi -> phi "cbor_pair_fst"; phi "cbor_pair_snd")
+}
+
+noextract
+let cbor_pair_td : C.typedef cbor_pair = Cs.struct_typedef cbor_pair_struct_def
+
+open Steel.ST.Util
+
+let test (#s: Ghost.erased cbor_case) (p: C.ref cbor_case_td)
+: ST (Ghost.erased cbor_case)
+    (C.pts_to p s)
+    (fun s' -> C.pts_to p s')
+    (C.full cbor_case_td s)
+    (fun s' -> C.full cbor_case_td s')
+= let ps = Cu.union_switch_field0 _ p "cbor_case_int64" (C.scalar U64.t) in
+  C.write ps 1729uL;
+  Cu.ununion_field p "cbor_case_int64" ps;
+  drop (Cu.has_union_field p "cbor_case_int64" _);
+  let s' = vpattern_replace (C.pts_to p) in
+  Cu.full_union cbor_case_union_def (Ghost.reveal s') "cbor_case_int64"; // FIXME: find a better pattern for that lemma
+  return _
